working on optimizations

tutorial/Asm.v
@@ -27,6 +27,8 @@ Typeclasses eauto := 5.
 (* end hide *)
 
 
+
+
 (** ** Syntax *)
 
 (** We define a countable set of memory addresses, represented as [string]s: *)
@@ -304,12 +306,23 @@ Definition interp_asm {E A} (t : itree (Reg +' Memory +' E) A) mem regs :
                                  (id_ _)) in
   let t' := interp h t
   in run_map (run_map t' regs) mem.
-  
+
 (** We can then define an evaluator for closed assembly programs by interpreting
     both store and heap events into two instances of [mapE], and running them
     both in the empty initial environments.  *)
-
 Definition eval_asm (p: asm unit void) := interp_asm (denote_asm p tt) empty empty.
+
+(* SAZ: Should some of thes notions of equivalence be put into the library?
+   SAZ: Should this be stated in terms of ktree ?
+ *)
+(** The definition [interp_asm] alos induces a notion of equivalence (open)
+    _asm_ programs *)
+Definition eq_asm_denotations {E A B} (t1 t2 : A -> itree (Reg +' Memory +' E) B) : Prop :=
+  forall (a:A) (mem:memory) (regs:registers),
+    (interp_asm (t1 a) mem regs) ≈ (interp_asm (t2 a) mem regs).
+
+Definition eq_asm {A B} (p1 p2 : asm A B) : Prop :=
+  eq_asm_denotations (denote_asm p1) (denote_asm p2).
 
 Section InterpAsmProperties.
 
