tutorial/AsmOptimization.v
@@ -1,5 +1,5 @@
 (* begin hide *)
-Require Import Asm Imp2AsmCorrectness Utils_tutorial.
+Require Import Asm AsmCombinators Imp2AsmCorrectness Utils_tutorial.
 
 Require Import Psatz.
 
@@ -15,7 +15,8 @@ From ITree Require Import
      ITree
      ITreeFacts
      Events.StateFacts
-     Events.Map.
+     Events.Map
+     Events.State.
 
 Import ITreeNotations.
 
@@ -31,59 +32,34 @@ Open Scope string_scope.
 (* end hide *)
 
 
+
+
 (* optimizations ------------------------------------------------------------ *)
 
-(* An optimization is just a function from asm units to asm units. *)
+(** A (simple) optimization is just a function from asm units to asm units. *)
 
 Definition optimization {A B} := asm A B -> asm A B.
 
-(* An optimization is correct if it yields an equivalent computation.
+(** An optimization is correct if it yields an equivalent computation.
 
-    - Note that AsmEval requires that resulting local environment and 
+    - Note that eq_asm requires that resulting register environment and 
       the resulting heap must be equivalent, so this formulation of
       correctness does not permit the elimination of local variables or
-      changes to the state. We could relax this definition (and thereby
-      allow more optimizations to be considered correct. 
+      differences in the state.  Those optimizations would require
+      more contextual information.
 *)
-Definition optimization_correct (opt:optimization) :=
-  forall (p : asm unit void),
-    AsmEval p ≈ AsmEval (opt p).
+Definition optimization_correct A B (opt:optimization) :=
+  forall (p : asm A B),
+    eq_asm p (opt p).
 
 
 (* peephole optimizations --------------------------------------------------- *)
 
-(* A (simple) peephole optmization transforms one instruction into a 
+(** A (simple) peephole optmization transforms one instruction into a 
    (possibly empty) list of equivalent instructions. *)
 Definition peephole_optimization := instr -> list instr.
 
-
-(* SAZ: this code for appending a list of instructions at the beginning of a block 
-   could be useful elsewhere.  We need it to define what it means to apply a 
-   peephole optimization to each instruction in a block. *)
-Fixpoint blk_append {lbl} (l:list instr) (b:block lbl) : block lbl :=
-  match l with
-  | [] => b
-  | i :: l' => bbi i (blk_append l' b)
-  end.
-
-(* TODO: Use the AsmCombinators Here... *)
-(* TODO: generalize effect type *)
-Fixpoint denote_instr_list (l:list instr) : itree (Locals +' Memory +' Exit) unit :=
-  match l with
-  | [] => ret tt
-  | i::l' => denote_instr i ;; denote_instr_list l'
-  end.
-
-Lemma denote_blk_append : forall lbl (l:list instr) (b:block lbl),
-    denote_block (blk_append l b) ≈ (x <- denote_instr_list l ;; denote_block b).
-Proof.
-  intros lbl.
-  induction l; intros b; simpl.
-  - rewrite bind_ret. reflexivity.
-  - rewrite bind_bind.
-    apply eutt_bind. red. intros. apply IHl. reflexivity.
-Qed.    
-
+(** We lift peephole optimizations to _asm_ pointwise through the structures. *) 
 Fixpoint peephole_optimize_block {lbl} (ph : peephole_optimization) (b:block lbl) : block lbl :=
   match b with
   | bbi i k => blk_append (ph i) (peephole_optimize_block ph k)
@@ -97,33 +73,41 @@ Definition peephole_optimize_asm {A B} (ph : peephole_optimization) (p : asm A B
   Build_asm A B (p.(internal)) (peephole_optimize_bks ph (p.(code))).
 
 
-(* SAZ: for now, we explicitly define the handler context in which the optimization will be considered correct.
-   
-*)
-Definition h : Handler (Locals +' Memory +' Exit)  ((mapE Imp.var Imp.value) +' ((mapE Imp.var Imp.value) +' Exit)) :=
-  (bimap evalLocals (bimap evalMemory (id_ _))).
+(* peephole correctness ----------------------------------------------------- *)
 
-Check run_map.
+Section Correctness.
 
-Definition ph_correct (ph : peephole_optimization) :=
-  forall i e1 e2,
-    
-    run_map (interp h (denote_instr i)) e ≈ run_map (interp h (denote_instr_list (ph i))) e.
+  (* SAZ: Should we set this this here?? *)
 
-Lemma ph_correct_append : forall (ph : peephole_optimization) (H : ph_correct ph)
-  lbl b1 b2 i,
-    interp h (denote_block b1) ≈ interp h ((denote_block b2) : itree (Locals +' Memory +' Exit) lbl)  ->
-    interp h (denote_instr i ;; denote_block b1) ≈ interp h (denote_block (blk_append (ph i) b2)).
-Proof.
-  intros ph H lbl b1 b2 i HP.
-  rewrite denote_blk_append.
-  unfold ph_correct in H.
-  rewrite interp_bind.
-  rewrite H.
-  rewrite interp_bind.
-  apply eutt_bind. red.  intros. apply HP.
-  reflexivity.
-Qed.  
+  (** A peephole optimizer is correct if it replaces an instruction with 
+    a semantically equivalent sequence of instructions. *)
+  Definition ph_correct (ph : peephole_optimization) :=
+  forall (i:instr),
+    @eq_asm_denotations Exit unit _ (fun _ => denote_instr i) (fun _ => denote_list (ph i)).
+
+  Lemma ph_blk_append_correct : forall (ph : peephole_optimization) (H : ph_correct ph)
+    lbl b1 b2 i,
+    (@eq_asm_denotations Exit unit lbl (fun _ => denote_block b1) (fun _ => denote_block b2)) ->
+    (@eq_asm_denotations Exit unit lbl
+                         (fun _ => denote_instr i ;; denote_block b1)
+                         (fun _ => denote_block (blk_append (ph i) b2))).
+  Proof.
+    intros ph H lbl b1 b2 i HP.
+    unfold eq_asm_denotations.
+    intros a mem regs. 
+    rewrite denote_blk_append.
+    unfold ph_correct in H.
+    unfold eq_asm_denotations in H.
+    specialize H with (i:=i).
+    pose proof (H a) as H2.
+    do 2 rewrite interp_asm_bind.
+    eapply eutt_clo_bind.
+    apply H2.
+    intros. subst.
+    destruct u2 as [g [l ?]].
+    apply HP.
+    exact tt.
+  Qed.  
 
 
 Lemma peephole_block_correct : 
@@ -131,102 +115,138 @@ Lemma peephole_block_correct :
     (H : ph_correct ph)
     lbl
     (b : block lbl),
-          (interp h ((denote_block b) : itree (Locals +' Memory +' Exit) lbl)) ≈
-          (interp h (denote_block (peephole_optimize_block ph b) : itree (Locals +' Memory +' Exit) lbl)).
+    @eq_asm_denotations Exit unit lbl
+                        (fun _ => denote_block b)
+                        (fun _ => denote_block (peephole_optimize_block ph b)).
 Proof.
   intros ph H lbl b.
   induction b.
-  - unfold h in *.
-    simpl.
-    rewrite ph_correct_append.
-    reflexivity.
-    assumption.
-    apply IHb.
-  - reflexivity.
+  - simpl.
+    unfold eq_asm_denotations.
+    intros.
+    apply ph_blk_append_correct; auto.
+  - unfold eq_asm_denotations.
+    intros. reflexivity.
 Qed.    
 
-Lemma peephole_optimization_correct : forall (ph : peephole_optimization) (H : ph_correct ph),
-    optimization_correct (peephole_optimize_asm ph).
+Lemma peephole_optimization_correct : forall A B (ph : peephole_optimization) (H : ph_correct ph),
+    optimization_correct A B (peephole_optimize_asm ph).
 Proof.
-  intros ph H.
+  intros A B ph H.
   unfold optimization_correct.
   intros p.
-  destruct p.
+  destruct p. 
   unfold peephole_optimize_asm.
   simpl.
-  unfold peephole_optimize_bks.
-  simpl.
-  unfold AsmEval.
-  apply eutt_interp_state; auto.
-  apply eutt_interp_state; auto.
+  unfold eq_asm, eq_asm_denotations.
+  intros.
   unfold denote_asm.
-  rewrite interp_loop.
-  rewrite interp_loop.
+  unfold interp_asm.
+  unfold run_map.
+  apply eutt_interp_state; auto.
+  apply eutt_interp_state; auto.
+  (* SAZ: The existential types for internal labels used in [asm] seem to be the source 
+     universe inconsistency problems.  I would like to just do [rewrite interp_loop], but
+     that fails with a (hidden) unification error, which seems to stem from the error
+     exhibited by the following.
+   *)
+  epose proof interp_loop.
+  red in H0.
+  unfold denote_b.
+  simpl.
+  Fail rewrite (H0 (bimap eval_reg (bimap eval_memory (id_ Exit))) _ _ internal).
+(*
   apply eutt_loop.
   simpl. red. intros. 
   unfold denote_b.
   apply peephole_block_correct.
   assumption.
 Qed.
+ *)
+Admitted.  
 
 
 (* concrete optimizations --------------------------------------------------- *)
 
 Definition simple (i:instr) : list instr :=
   match i with
-  | Imov dest (Ovar src) =>
-    if dest =? src then [] else [i]
+  | Imov dest (Oreg src) =>
+    if Nat.eqb dest src then [] else [i]
   | _ => [i]
   end.
 
 
-Lemma interp_h_ret_tt : forall (t : itree (Locals +' Memory +' Exit) unit),
-    interp h t ≈ interp h (t ;; Ret tt).
+Lemma interp_asm_ret_tt : forall (t : itree (Reg +' Memory +' Exit) unit) mem regs,
+    interp_asm t mem regs ≈ interp_asm (t ;; Ret tt) mem regs.
 Proof.
-  intros t.
-  rewrite interp_bind.
+  intros t mem regs.
+  rewrite interp_asm_bind.
   rewrite <- bind_ret2 at 1.
-  apply eutt_bind. red.  intros. destruct a. rewrite interp_ret. reflexivity.
-  reflexivity.  
+  eapply eutt_clo_bind. reflexivity.
+  intros. subst. unfold interp_asm.
+  destruct u2 as [g [l x]].
+  unfold run_map.
+  rewrite interp_ret.
+  do 2 rewrite interp_state_ret.
+  destruct x.
+  reflexivity.
 Qed.
-
 
 
 Lemma simple_correct : ph_correct simple.
 Proof.
   unfold ph_correct.
   intros i.
-  destruct i; simpl.
+  unfold eq_asm_denotations. intros. 
+  destruct i; simpl; try apply interp_asm_ret_tt.
   - destruct src.
-    + simpl. rewrite bind_ret. apply interp_h_ret_tt. 
+    + simpl. rewrite bind_ret.
+      apply interp_asm_ret_tt. 
     + simpl.
-      destruct (string_dec dest v).
-      * subst.
-        rewrite String.eqb_refl.
-        simpl. 
+      destruct (Nat.eq_dec dest r).
+      * subst. 
+        rewrite Nat.eqb_refl.
+        simpl.
+        unfold interp_asm, run_map.
         rewrite interp_ret.
+        do 2 rewrite interp_state_ret.
         rewrite interp_bind.
         rewrite interp_trigger.
         rewrite bind_tau.
         rewrite tau_eutt.
-        unfold h.
+        do 2 rewrite interp_state_bind.
         cbn.
-                
+        unfold CategoryOps.cat, Cat_Handler, Handler.cat. simpl.
+        unfold lookup_def.
+        repeat rewrite interp_bind.
+        setoid_rewrite interp_ret.
+        repeat rewrite interp_state_bind.
+        repeat rewrite bind_bind.        
+        repeat setoid_rewrite interp_state_ret.
 
-        About CategoryOps.cat. unfold CategoryOps.cat, Cat_Handler, Handler.cat. simpl. 
-        unfold lookup_def. rewrite interp_bind. unfold Map.lookup, embed, Embeddable_forall, embed, Embeddable_itree . rewrite interp_trigger.
-        rewrite bind_bind. rewrite bind_tau. rewrite tau_eutt.
+        unfold Map.lookup.
+        unfold embed, Embeddable_itree, Embeddable_forall, inl_, embed.
+        rewrite interp_trigger. rewrite tau_eutt.
+        unfold Inl_sum1_Handler, Handler.inl_, Handler.htrigger.
+        rewrite interp_state_trigger. rewrite tau_eutt.
+        cbn.
+        rewrite interp_state_ret.
+        repeat rewrite bind_ret.
+        simpl.
+        rewrite interp_trigger.
+        rewrite tau_eutt.
+        cbn. 
+        unfold CategoryOps.cat, resum, ReSum_id, id_, eval_reg, inl_. cbn.
+        setoid_rewrite interp_trigger. rewrite tau_eutt.
+        rewrite interp_state_trigger.
+        rewrite tau_eutt.
+        cbn.
+        rewrite interp_state_ret.
+
+        (* SAZ: need to propagate an equivalence relation on the register state. *)
+
         
-        
-        (* SAZ: Not sure what the right way to progress here is. *)
-        SearchAbout bimap.
-        admit.
-        
-      * apply String.eqb_neq in n. rewrite n.
-        simpl. apply interp_h_ret_tt.
-  - apply interp_h_ret_tt.
-  - apply interp_h_ret_tt.
-  - apply interp_h_ret_tt.
-  - apply interp_h_ret_tt.
-  - apply interp_h_ret_tt.    
 Admitted.    
+
+
+End Correctness.
